Click/MG.v
@@ -1,0 +1,392 @@
+Require Import Base.
+Require Import Circuit.
+Require Import StateSpace.
+Require Import Monad.
+
+Require Import List.
+Import ListNotations.
+Open Scope list_scope.
+
+Require Import MarkedGraph.
+Require Import Click.StateSpace.
+Require Import Click.Invariants.
+
+
+Require Import Omega.
+
+
+Import EnsembleNotation.
+Open Scope ensemble_scope.
+Require Import Coq.Program.Equality.
+
+Module ClickMG (ClickModule : ClickType).
+  Export ClickModule.
+  Module Desync := Desync(ClickModule).
+  Export Desync.
+  Module WFClick := WFStage(ClickModule).
+  Export WFClick.
+  Module SSTactics := StateSpaceTactics(Name).
+  Export SSTactics.
+
+Section TokenMG.
+
+  Inductive token_transition :=
+  | left_ack : token_transition
+  | left_req : token_transition
+  | right_req
+  | right_ack
+  | clk_rise
+  | clk_fall
+  .
+  Instance token_transition_eq_dec : eq_dec token_transition.
+  Proof.
+    constructor; intros x y;
+    destruct x; destruct y;
+      try (left; reflexivity); try (right; discriminate).
+  Defined.
+
+
+  (***TODO: See ipad notes, removing timing assumptions here and replace with clk_fall
+  → left_ack assumption. Also TODO: incorporate this delay into state space Click controller. *)
+
+  Inductive stage_place : token_transition -> token_transition -> Set :=
+  (* L.ack -> L.req *)
+  (* CLK- -> L.req *)
+  (* R.req -> L.req *)
+  (* ENVIRONMENT constraint: we expect handshakes to obey a 2-phase handshake
+     protocol, so we don't expect an input on left_req until left_ack has been
+     updated by the controller. *)
+  | left_ack_left_req : stage_place left_ack left_req
+  (* TIMING constraint: changes inside the controller propogate faster than
+     communication between controllers. In the controller, if this is not
+     respected, it will lead to an error state as the clock component will not
+     be stable when the new inputs arrive. *)
+  | clk_fall_left_ack : stage_place clk_fall left_ack
+  (* TIMING constraint: changes inside the controller propogate faster than
+     communication between controllers. In other words, wait for state0 to be
+     propogated to both left_ack AND right_req before accepting input on
+     left_req. *)
+
+  (* CLK+ -> L.ack *)
+  (* REDUNDANT
+  | clk_rise_left_ack : stage_place clk_rise left_ack
+  *)
+  
+  (* CLK+ -> R.req *)
+  | clk_rise_right_req : stage_place clk_rise right_req
+
+  (* R.req -> R.ack *)
+  (* ENVIRONMENT constraint: we expect handshakes to obey a 2-phase handshake
+     protocol, so we don't expect an input on right_ack until right_req has been
+     updated by the controller  *)
+  | right_req_right_ack : stage_place right_req right_ack
+  
+  (* CLK+ -> CLK- *)
+  | clock_fall : stage_place clk_rise clk_fall
+  (* REDUNDANT
+  | clock_rise : stage_place clk_fall clk_rise
+  *)
+  
+  (* left_req -> CLK+ *)
+  (* right_ack -> CLK+ *)
+  | left_req_clk_rise : stage_place left_req clk_rise
+  | right_ack_clk_rise : stage_place right_ack clk_rise
+  .
+
+
+  (** The only thing that is affected by token or non-token stages is the
+  initial markings. These are indexed by two boolean values: whether the current
+  stage has received a token or not on reset, and whether the current stage
+  generates a token or not on reset. *)
+
+
+  Definition init_marking_flag (in_flag : token_flag) (out_flag : token_flag) 
+      : forall t1 t2, stage_place t1 t2 -> nat :=
+    match in_flag, out_flag with
+    (* Traditional non-token stage *)
+    | Token, NonToken => fun t1 t2 p => match p with
+                                      | left_req_clk_rise => 1
+                                      | right_ack_clk_rise => 1
+(*                                      | clock_rise => 1*)
+                                      | _ => 0
+                                      end
+    (* Traditional token stage *)
+    | NonToken, Token => fun t1 t2 p => match p with
+                                        | left_ack_left_req => 1
+                                        | right_req_right_ack => 1
+(*                                        | clock_rise => 1*)
+                                        | _ => 0
+                                        end
+    (* Token with left token stage *)
+    | Token, Token    => fun t1 t2 p => match p with
+                                      | left_req_clk_rise => 1
+                                      | right_req_right_ack => 1
+(*                                      | clock_rise => 1*)
+                                      | _ => 0
+                                      end
+    | NonToken, NonToken => fun t1 t2 p => match p with
+                                           | left_ack_left_req => 1
+                                           | right_ack_clk_rise => 1
+(*                                           | clock_rise => 1*)
+                                           | _ => 0
+                                      end
+    end.
+
+  Variable in_flag out_flag : token_flag.
+
+  Definition stage_MG : marked_graph token_transition :=
+    {| place := stage_place
+     ; init_marking := init_marking_flag in_flag out_flag
+     |}.
+
+End TokenMG.
+
+Existing Instance token_transition_eq_dec.
+Arguments MG_SS {name name_dec transition transition_dec} MG {MG_scheme}.
+
+  Inductive place_eq : forall {t1 t2 t1' t2' : token_transition}, stage_place t1 t2 -> stage_place t1' t2' -> Prop :=
+  | place_refl : forall t1 t2 (p : stage_place t1 t2), place_eq p p.
+
+
+  Class stage_naming_scheme :=
+    { stage_place_name : forall (l : latch even odd) {t1 t2 : token_transition}, stage_place t1 t2 -> name
+    ; stage_places_disjoint_transitions : forall l t1 t2 (p : stage_place t1 t2),
+      stage_place_name l p ∉ space_domain (latch_stage_with_env l)
+    ; stage_places_all_disjoint : forall l f1 f2 {t1 t2 t1' t2'} (p : stage_place t1 t2) (p' : stage_place t1' t2'),
+      stage_place_name l p = stage_place_name l p' ->
+      StateSpace.place_eq (stage_MG f1 f2) p p'
+
+    }.
+
+  Instance stage_scheme : stage_naming_scheme :=
+    {| stage_place_name := fun l t1 t2 p =>
+                             match p with
+                             | left_ack_left_req => local_name l "left_ack_left_req"
+                             | clk_fall_left_ack => local_name l "clk_fall_left_ack"
+                             | clk_rise_right_req => local_name l "clk_rise_right_req"
+                             | right_req_right_ack => local_name l "right_req_right_ack"
+                             | clock_fall => local_name l "clock_fall"
+                             | left_req_clk_rise => local_name l "left_req_clk_rise"
+                             | right_ack_clk_rise => local_name l "right_ack_clk_rise"
+                             end
+    |}.
+  * intros l ? ? p.
+    Search space_domain latch_stage_with_env.
+    rewrite dom_latch_stage_with_env.
+    to_in_list_dec.
+    simpl.
+    destruct p; auto.
+  * intros l f1 f2 ? ? ? ? p p' Heq.
+    destruct p; destruct p'; find_contradiction;
+      constructor.
+  Defined.
+
+
+Section TokenMG_to_SS.
+
+  Variable l : latch even odd.
+  Variable in_flag : token_flag.
+  Let out_flag := latch_to_token_flag l.
+
+  Definition name_to_stage_place (x : name) : option { t1 : token_transition &
+                                                     { t2 : token_transition & stage_place t1 t2 }}.
+    refine (if x =? stage_place_name l left_ack_left_req
+            then Some (existT _ _ (existT _ _ left_ack_left_req))
+            else if x =? stage_place_name l clk_fall_left_ack
+            then Some (existT _ _ (existT _ _ clk_fall_left_ack))
+            else if x =? stage_place_name l clk_rise_right_req
+            then Some (existT _ _ (existT _ _ clk_rise_right_req))
+            else if x =? stage_place_name l right_req_right_ack
+            then Some (existT _ _ (existT _ _ right_req_right_ack))
+            else if x =? stage_place_name l clock_fall
+            then Some (existT _ _ (existT _ _ clock_fall))
+            else if x =? stage_place_name l left_req_clk_rise
+            then Some (existT _ _ (existT _ _ left_req_clk_rise))
+            else if x =? stage_place_name l right_ack_clk_rise
+            then Some (existT _ _ (existT _ _ right_ack_clk_rise))
+            else None).
+  Defined.
+  Lemma name_to_stage_place_eq : forall x t1 t2 (p : stage_place t1 t2),
+    name_to_stage_place x = Some (existT _ _ (existT _ _ p)) ->
+    x = stage_place_name l p.
+  Proof.
+    intros x t1 t2 p; destruct p; simpl; intros Heq;
+      unfold name_to_stage_place in Heq;
+      repeat compare_next; auto.
+  Qed.
+  Lemma name_to_stage_place_neq : forall x,
+    name_to_stage_place x = None ->
+    forall t1 t2 (p : stage_place t1 t2), x <> stage_place_name l p.
+  Proof.
+    intros x Heq.
+    unfold name_to_stage_place in Heq.
+    repeat compare_next.
+    intros t1 t2 p; destruct p; auto.
+  Qed.
+
+  Definition name_is_stage_place_dec x : 
+                           {t1 : token_transition &
+                           {t2 : token_transition & {p : stage_place t1 t2 & x = stage_place_name l p}}}
+                        + {forall t1 t2 (p : stage_place t1 t2), x <> stage_place_name l p}.
+    destruct (name_to_stage_place x) as [[t1 [t2 p]] | ] eqn:Hx.
+    * left. exists t1; exists t2; exists p.
+      apply name_to_stage_place_eq; auto.
+    * right. apply name_to_stage_place_neq; auto.
+  Defined.
+
+  Definition token_transition_update_value (t : token_transition) (v : value) : value :=
+    match t with
+    | clk_rise => Bit1
+    | clk_fall => Bit0
+    | _ => neg_value v
+    end.
+  Definition token_transition_name (t : token_transition) : name :=
+    match t with
+    | left_ack => ack (latch_input l)
+    | left_req => req (latch_input l)
+    | right_req => req (latch_output l)
+    | right_ack => ack (latch_output l)
+    | clk_rise  => latch_clk l
+    | clk_fall  => latch_clk l
+    end.
+  Lemma token_name_domain : forall t, token_transition_name t ∈ space_domain (latch_stage l).
+  Proof.
+    intros t.
+    unfold space_domain.
+    rewrite latch_stage_input, latch_stage_output.
+    destruct t; simpl; solve_set.
+  Qed.
+    
+
+  Program Instance stage_MG_scheme : MG_naming_scheme name (stage_MG in_flag out_flag) :=
+  {| transition_name := token_transition_name
+   ; place_name := @stage_place_name _ l
+   ; name_to_place := name_to_stage_place
+   ; transition_update_value := token_transition_update_value
+   ; input_transition := from_list [left_req; right_ack]
+   |}.
+  Next Obligation.
+    split; intros Hx.
+    { apply name_to_stage_place_eq in Hx; subst. reflexivity. }
+    { destruct p; subst; simpl; unfold name_to_stage_place; simpl; reduce_eqb; reflexivity. }
+  Qed.
+  Next Obligation.
+    destruct p; destruct t; inversion 1.
+  Qed.
+  Next Obligation.
+    decompose_set_structure; destruct t'; find_contradiction; auto.
+  Qed.
+  Next Obligation.
+    destruct p; destruct p'; find_contradiction;
+      constructor.
+  Qed.
+
+  Definition stage_MG_SS : StateSpace name := MG_SS (stage_MG in_flag out_flag).
+
+  Definition transition_event (t : token_transition) (σ : state name) : event name value :=
+    let x := @transition_name name _ (stage_MG in_flag out_flag) _ t in
+    let v := @transition_update_value name _ (stage_MG in_flag out_flag) _ t (σ x) in
+    Event x v.
+
+
+End TokenMG_to_SS.
+Existing Instance stage_MG_scheme.
+About name_to_place.
+Arguments name_to_place {name transition} MG {MG_naming_scheme}.
+Arguments traces_of {name}.
+
+
+  Section SS_to_TokenMG.
+
+  Variable l : latch even odd.
+  Let out_flag := latch_to_token_flag l.
+  (* in_flag is opposite of out_flag here *)
+  Let in_flag := swap_token_flag (latch_to_token_flag l).
+
+  Definition init_stage_MG_state : state name.
+  Proof.
+    intros x.
+    refine (if x =? stage_place_name l left_ack_left_req
+            then Num (init_marking (stage_MG in_flag out_flag) _ _ left_ack_left_req)
+            else if x =? stage_place_name l clk_fall_left_ack
+            then Num (init_marking (stage_MG in_flag out_flag) _ _ clk_fall_left_ack)
+            else if x =? stage_place_name l clk_rise_right_req
+            then Num (init_marking (stage_MG in_flag out_flag) _ _ clk_rise_right_req)
+            else if x =? stage_place_name l right_req_right_ack
+            then Num (init_marking (stage_MG in_flag out_flag) _ _ right_req_right_ack)
+            else if x =? stage_place_name l clock_fall
+            then Num (init_marking (stage_MG in_flag out_flag) _ _ clock_fall)
+            else if x =? stage_place_name l left_req_clk_rise
+            then Num (init_marking (stage_MG in_flag out_flag) _ _ left_req_clk_rise)
+            else if x =? stage_place_name l right_ack_clk_rise
+            then Num (init_marking (stage_MG in_flag out_flag) _ _ right_ack_clk_rise)
+            else (σR l x)).
+  Defined.
+
+
+  Lemma dom_MG_SS : space_domain (stage_MG_SS l in_flag)
+               == from_list [ token_transition_name l left_ack
+                            ; token_transition_name l left_req
+                            ; token_transition_name l right_req
+                            ; token_transition_name l right_ack
+                            ; token_transition_name l clk_rise
+                            ; token_transition_name l clk_fall
+
+                            ; stage_place_name l left_ack_left_req
+                            ; stage_place_name l clk_fall_left_ack
+                            ; stage_place_name l clk_rise_right_req
+                            ; stage_place_name l right_req_right_ack
+                            ; stage_place_name l clock_fall
+                            ; stage_place_name l left_req_clk_rise
+                            ; stage_place_name l right_ack_clk_rise
+                            ].
+  Proof.
+    unfold space_domain. constructor; intros x Hx.
+    * to_in_list_dec. simpl. simpl in Hx.
+      deep_decompose_set_structure; simpl; reduce_eqb; auto;
+        subst;
+        match goal with
+        | [ |- context[ token_transition_name _ ?t =? _ ] ] =>
+          destruct t; simpl; reduce_eqb; auto
+        | [ |- context[ place_name ?p =? _ ] ] =>
+          destruct p; simpl; reduce_eqb; auto
+        end.
+    * to_in_list_dec. unfold in_list_dec in Hx.
+      simpl.
+      repeat compare_next;
+        try (left; left; eexists; split; [ | reflexivity]; solve_set);
+        try (left; right; eexists; split; [ | reflexivity]; solve_set);
+        try (right; do 3 eexists; reflexivity).
+  Qed. 
+
+  Lemma stage_internal_disjoint :
+    space_internal (latch_stage_with_env l) ⊥ space_domain (stage_MG_SS l in_flag).
+  Proof.
+    rewrite latch_stage_with_env_internal.
+    rewrite dom_MG_SS.
+    simpl.
+    constructor; intros x [? Hx Hy].
+    contradict Hy.
+    decompose_set_structure;
+      solve_space_set.
+  Qed.
+  Lemma stage_MG_internal_disjoint :
+    space_internal (stage_MG_SS l in_flag) ⊥ space_domain (latch_stage_with_env l).
+  Proof.
+    rewrite dom_latch_stage_with_env. simpl.
+    constructor. intros x [? Hx Hy].
+    contradict Hy.
+    destruct Hx as [t1 [t2 [p Hp]]]; subst.
+    destruct p; solve_space_set.
+  Qed.
+
+End SS_to_TokenMG.
+
+Hint Resolve stage_internal_disjoint stage_MG_internal_disjoint : click.
+Hint Resolve wf_MG_SS : click.
+Arguments well_formed {name}.
+Arguments stage_place_name {stage_naming_scheme} l {t1 t2}.
+Arguments place_name {name transition} MG {MG_naming_scheme} {t1 t2}.
+
+
+End ClickMG.
